theories/Compositional_Structures/Basic_Modules/Plurality_Module_Ref.thy
@@ -1,7 +1,7 @@
 theory Plurality_Module_Ref
   imports 
         "Verified_Voting_Rule_Construction.Plurality_Module"
-        "Component_Types/Social_Choice_Types/Counting_Functions_Code"
+        "Component_Types/Social_Choice_Types/Profile_List_Monadic"
         "Component_Types/Electoral_Module_Ref"
     
 begin
@@ -28,12 +28,14 @@ definition "scoremax A scores \<equiv> do {
     }) (0::nat)
 }"
 
-definition "pluralityparam A scores threshold \<equiv>
+definition pluralityparam ::
+    "'a set \<Rightarrow> ('a \<Rightarrow> nat option) \<Rightarrow> nat \<Rightarrow> 'a Result nres" where 
+"pluralityparam A scores threshold \<equiv>
     FOREACH (A)
     (\<lambda>x (e,r,d). do {
       ASSERT (x \<in> dom scores);
       let scx = the (scores x);
-      sel \<leftarrow> threshold;
+      let sel = threshold;
       (if (scx = sel) then 
           RETURN (insert x e,r,d) 
       else 
@@ -45,7 +47,8 @@ definition "pluralityparam A scores threshold \<equiv>
 definition plurality_init:: "'a Electoral_Module_Ref" where 
 "plurality_init A p \<equiv> do {
   scores <- compute_scores A p;
-  pluralityparam A scores (scoremax A scores)
+  threshold <- (scoremax A scores);
+  pluralityparam A scores threshold
 }"
 
 sepref_definition plurality_sepref is
@@ -68,25 +71,26 @@ begin
 
 definition "precompute_map \<equiv> (\<lambda>a. Some (win_count pr a))|`A"
 
-definition "max_comp_spec_plurality \<equiv> 
-(SPEC (\<lambda>max. (\<forall>a \<in> A. win_count pr a \<le> max) \<and> ((\<exists>e \<in> A. max = win_count pr e) \<or> max = 0)))"
+definition "max_comp_plurality \<equiv> Max {win_count pr x |x. x \<in> A}"
 
 lemma plurality_monadic_correct:
-  shows "(pluralityparam A precompute_map max_comp_spec_plurality
+  shows "(pluralityparam A precompute_map max_comp_plurality
            ,(SPEC (\<lambda> elecres. elecres = plurality A pr))) \<in> \<langle>Id\<rangle>nres_rel "
-  unfolding pluralityparam_def precompute_map_def max_comp_spec_plurality_def
+  unfolding pluralityparam_def precompute_map_def max_comp_plurality_def
   apply (refine_vcg FOREACH_rule[where I = 
         "(\<lambda>it (e,r,d). (\<forall>elem \<in> e.  \<forall>a \<in> A. win_count pr a \<le> win_count pr elem)
           \<and> (\<forall>elem \<in> r.  \<exists>a \<in> A. win_count pr a > win_count pr elem)
           \<and> d = {} 
           \<and> e \<union> r = (A - it))"] )
-  apply (auto simp add: fina
+  apply (clarsimp_all simp add: fina
     simp del: win_count.simps )
-  using nat_less_le apply blast
+  subgoal by auto
+  using fina nbmax[where A= A and p = pr and f=win_count]
+  using fina nempa nbexmax[where A= A and p = pr and f=win_count] 
   apply (rename_tac e r alt)
-  using leD apply blast
-   apply (metis UnCI leD)+
-  done
+  using leD 
+   (*apply (metis UnCI leD)+*)
+  sorry
 
 
 lemma compute_scores_correct:
@@ -122,27 +126,31 @@ qed
 
 
 lemma scoremax_correct:
-  shows "(scoremax A precompute_map, max_comp_spec_plurality) \<in> \<langle>nat_rel\<rangle>nres_rel"
-  unfolding scoremax_def max_comp_spec_plurality_def precompute_map_def
+  shows "(scoremax A precompute_map, SPEC (\<lambda> th. th =  max_comp_plurality)) \<in> \<langle>nat_rel\<rangle>nres_rel"
+  unfolding scoremax_def max_comp_plurality_def precompute_map_def
   apply (refine_vcg FOREACH_rule[where I = "(\<lambda>it max. (\<forall>a \<in> (A - it). win_count pr a \<le> max) \<and> ((\<exists>e \<in> (A - it). max = win_count pr e) \<or> max = 0))"] )
   apply (auto simp add: fina simp del: win_count.simps)
   apply (metis Diff_iff leD nle_le order_trans)
-  apply (metis DiffI order_less_imp_le)
+    apply (metis DiffI order_less_imp_le)
+  using fina nbmax[where A= A and p = pr and f=win_count]
+  nempa nbexmax[where A= A and p = pr and f=win_count]
+  apply (metis antisym linorder_not_le max_comp_plurality_def)
+  using fina nempa nbexmax[where A= A and p = pr and f=win_count]
+  apply (simp add: finite_nat_set_iff_bounded)
   done
 
 lemma parameterized_refinement: 
-  "(pluralityparam, pluralityparam) \<in> \<langle>Id\<rangle>set_rel \<rightarrow> Id \<rightarrow> \<langle>nat_rel\<rangle>nres_rel \<rightarrow> \<langle>Id\<rangle>nres_rel"
+  "(pluralityparam, pluralityparam) \<in> \<langle>Id\<rangle>set_rel \<rightarrow> Id \<rightarrow> nat_rel \<rightarrow> \<langle>Id\<rangle>nres_rel"
   unfolding pluralityparam_def
   apply (refine_vcg)
-  apply (refine_dref_type)
   apply (auto simp add: refine_rel_defs)[3]
   apply clarsimp_all
-  using nres_relD refine_IdD by blast
+  done
 
 
-lemma rewritep: "((RETURN precompute_map) \<bind> 
+(*lemma rewritep: "((RETURN precompute_map) \<bind> 
 (\<lambda> map. pluralityparam A map (scoremax A map)), 
-pluralityparam A precompute_map max_comp_spec_plurality)
+pluralityparam A precompute_map max_comp_plurality)
   \<in> \<langle>Id\<rangle>nres_rel"
   apply clarsimp
   apply refine_vcg
@@ -158,40 +166,56 @@ proof -
     apply (refine_dref_type)
     apply (auto simp add: refine_rel_defs)
     using refi refine_IdD by blast
-qed
+qed*)
 
 
-lemma scores_param: "(compute_scores A pl \<bind> (\<lambda> map. pluralityparam A map 
-  (scoremax A map)), pluralityparam A precompute_map max_comp_spec_plurality)
+(*lemma scores_param: "(compute_scores A pl \<bind> (\<lambda> map. pluralityparam A map 
+  (scoremax A map)), pluralityparam A precompute_map max_comp_plurality)
   \<in> \<langle>Id\<rangle>nres_rel"
   using rewritep compute_scores_correct in_nres_rel_iff
   by (metis (no_types, lifting) BNF_Greatest_Fixpoint.IdD Collect_cong Id_refine 
-SPEC_eq_is_RETURN(2) bind_refine conc_trans_additional(5)) 
-  
+SPEC_eq_is_RETURN(2) bind_refine conc_trans_additional(5)) *)
+
+find_theorems bind
 
 lemma plurality_init_refine:
-  shows "(plurality_init A pl, (pluralityparam A precompute_map max_comp_spec_plurality))
+  shows "(plurality_init A pl, (pluralityparam A precompute_map max_comp_plurality))
       \<in> \<langle>Id\<rangle>nres_rel"
-  unfolding plurality_init_def 
-  using scores_param nres_relD by blast 
+  apply (rule nres_relI)
+  apply (simp add: Id_refine)
+  unfolding plurality_init_def
+proof -
+  have "SPEC(\<lambda> map. map =precompute_map) \<bind> (\<lambda>scores. scoremax A scores \<bind> pluralityparam A scores)
+    \<le> pluralityparam A precompute_map max_comp_plurality"
+    using scoremax_correct[THEN nres_relD, THEN refine_IdD]
+    by (metis (no_types, lifting) Collect_cong RETURN_SPEC_conv Refine_Basic.bind_mono(1) let_to_bind_conv order_mono_setup.refl) 
+  from this show "compute_scores A pl \<bind> (\<lambda>scores. scoremax A scores \<bind> pluralityparam A scores)
+    \<le> pluralityparam A precompute_map max_comp_plurality"
+    using compute_scores_correct[THEN nres_relD, THEN refine_IdD]
+    using Refine_Basic.bind_mono(1) dual_order.trans by blast
+qed 
+  
 
-lemmas plurality_init_refspec = plurality_init_refine[FCOMP plurality_monadic_correct]
+(*lemmas plurality_init_refspec = plurality_init_refine[FCOMP plurality_monadic_correct]*)
 
 theorem plurality_init_correct:
   shows "(plurality_init A pl, (SPEC (\<lambda> elecres. elecres = plurality A pr)))
      \<in> \<langle>Id\<rangle>nres_rel"
-  apply(rule nres_relI) 
+  apply (rule nres_relI)
+  apply (rule refine_IdI)
+  using plurality_monadic_correct[THEN nres_relD, THEN refine_IdD]
   using ref_two_step[OF plurality_init_refine[THEN nres_relD] 
-            plurality_monadic_correct [THEN nres_relD]] refine_IdD
-  by fastforce   
+plurality_monadic_correct[THEN nres_relD, THEN refine_IdD], THEN refine_IdD]
+  by fastforce
+  
 
 theorem plurality_init_dataref:
   shows "(plurality_init, (\<lambda> Alts p. SPEC (\<lambda> elec. elec = (plurality) Alts p)))
      \<in> \<langle>Id\<rangle>set_rel \<rightarrow> (profile_rel) \<rightarrow> \<langle>Id\<rangle>nres_rel"
 
-  sorry
+  oops
 
-lemmas pluralitysep_correct= "plurality_sepref.refine[FCOMP plurality_init_dataref]"
+(*lemmas pluralitysep_correct= "plurality_sepref.refine[FCOMP plurality_init_dataref]"*)
 
 end
 
