theories/Compositional_Structures/Basic_Modules/Component_Types/Elimination_Module_Ref.thy
@@ -1,7 +1,7 @@
 section \<open>Elimination Module\<close>
 
 theory Elimination_Module_Ref
-  imports Verified_Voting_Rule_Construction.Evaluation_Function
+  imports Evaluation_Function_Ref
           Verified_Voting_Rule_Construction.Electoral_Module
 Refine_Imperative_HOL.IICF
 begin
@@ -19,15 +19,35 @@ type_synonym Threshold_Value = nat
 
 type_synonym Threshold_Relation = "nat \<Rightarrow> nat \<Rightarrow> bool"
 
-type_synonym 'a Electoral_Set = "'a set \<Rightarrow> 'a Profile \<Rightarrow> 'a set"
+type_synonym 'a Electoral_Set_Ref = "'a set \<Rightarrow> 'a Profile_List \<Rightarrow> 'a set nres"
 
-fun elimination_set :: "'a Evaluation_Function \<Rightarrow> Threshold_Value \<Rightarrow>
-                            Threshold_Relation \<Rightarrow> 'a Electoral_Set" where
- "elimination_set e t r A p = {a \<in> A . r (e a A p) t }"
+definition pre_compute_scores :: "'a Evaluation_Function_Ref \<Rightarrow>
+ 'a set \<Rightarrow> 'a Profile_List \<Rightarrow> ('a \<rightharpoonup> nat) nres" 
+  where "pre_compute_scores ef A p \<equiv>
+  FOREACH A 
+    (\<lambda>x m. do {
+      scx \<leftarrow> (ef x A p);
+      RETURN (m(x\<mapsto>scx))
+  }) (Map.empty)"
 
-fun elimination_module :: "'a Evaluation_Function \<Rightarrow> Threshold_Value \<Rightarrow>
+
+definition eliminate:: "'a Evaluation_Function_Ref \<Rightarrow> Threshold_Value \<Rightarrow>
+                            Threshold_Relation \<Rightarrow> 
+                          'a set \<Rightarrow> 'a Profile_List \<Rightarrow> ('a set \<times> 'a set) nres" where
+ "eliminate evaf t r A p \<equiv> do {
+   FOREACH (A)
+    (\<lambda>x (rej, def). do {
+      scx <- evaf x A p;
+      (if (r scx t) then 
+          RETURN (insert x rej, def) 
+      else 
+          RETURN(rej, insert x def))
+    }) ({}, {})
+}"
+
+definition elimination_module :: "'a Evaluation_Function \<Rightarrow> Threshold_Value \<Rightarrow>
                             Threshold_Relation \<Rightarrow> 'a Electoral_Module" where
-  "elimination_module e t r A p =
+  "elimination_module e t r A p \<equiv>
       (if (elimination_set e t r A p) \<noteq> A
         then ({}, (elimination_set e t r A p), A - (elimination_set e t r A p))
         else ({},{},A))"
