theories/Compositional_Structures/Basic_Modules/Component_Types/Social_Choice_Types/Result_Ref.thy
@@ -1,8 +1,0 @@
-theory Result_Ref
-  imports "Verified_Voting_Rule_Construction.Result"
-
-begin
-
-type_synonym 'a Result_Ref = "'a list * 'a list * 'a list"
-
-end
